src/hls/ClockRegisters.v
@@ -31,10 +31,11 @@ Require Import vericert.common.Vericertlib.
 Require Import vericert.hls.ValueInt.
 Require Import vericert.hls.AssocMap.
 Require Import vericert.hls.Array.
+Require Import vericert.hls.Verilog.
 Require Import vericert.hls.DHTL.
-Require vericert.hls.Verilog.
 
 Require Import vericert.common.Errormonad.
+Import Errors.
 Import ErrorMonad.
 Import ErrorMonadExtra.
 Import MonadNotation.
@@ -153,63 +154,216 @@ Definition expand_assignment (f: flat_stmnt): Verilog.stmnt :=
 Definition fold_seq_block (s: list flat_stmnt): Verilog.stmnt :=
   fold_left (fun a b => Verilog.Vseq a (expand_assignment b)) s Verilog.Vskip.
 
-Fixpoint clock_expr (t: PTree.t flat_expr) (f: flat_expr): flat_expr :=
+Fixpoint clock_flat_expr (t: PTree.t flat_expr) (f: flat_expr): flat_expr :=
   match f with
   | FVvar r => 
     match PTree.get r t with
     | Some e => e
     | None => FVvar r
     end
-  | FVunop b e => FVunop b (clock_expr t e)
+  | FVunop b e => FVunop b (clock_flat_expr t e)
   | FVbinop b e1 e2 => 
-    FVbinop b (clock_expr t e1) (clock_expr t e2)
+    FVbinop b (clock_flat_expr t e1) (clock_flat_expr t e2)
   | FVternary e1 e2 e3 => 
-    FVternary (clock_expr t e1) (clock_expr t e2) (clock_expr t e3)
+    FVternary (clock_flat_expr t e1) (clock_flat_expr t e2) (clock_flat_expr t e3)
   | _ => f
   end.
 
-Definition clock_assignment (tl: RTree.t flat_expr * list flat_stmnt) (f: flat_stmnt): 
-    (RTree.t flat_expr * list flat_stmnt) :=
-  let (t, l) := tl in
+Fixpoint clock_expr (t: PTree.t expr) (f: expr): res expr :=
   match f with
-  | FVblock r e => 
-    let fe := clock_expr t e in 
-    (PTree.set r fe t, l ++ (FVnonblock r fe :: nil))
-  | _ => (t, l ++ (f :: nil))
+  | Vvar r => 
+    match PTree.get r t with
+    | Some e => OK e
+    | None => OK (Vvar r)
+    end
+  | Vunop b e => do e' <- (clock_expr t e); OK (Vunop b e')
+  | Vbinop b e1 e2 => 
+    do e1' <- (clock_expr t e1);
+    do e2' <- (clock_expr t e2);
+    OK (Vbinop b e1' e2')
+  | Vternary e1 e2 e3 =>
+    do e1' <- (clock_expr t e1);
+    do e2' <- (clock_expr t e2);
+    do e3' <- (clock_expr t e3);
+    OK (Vternary e1' e2' e3')
+  | Vvari r e => do e' <- (clock_expr t e); OK (Vvari r e')
+  | Vrange r e1 e2 => Error (msg "ClockRegisters: could not translate Vrange")
+  | Vinputvar r => OK (Vinputvar r)
+  | Vlit v => OK (Vlit v)
   end.
 
-Definition clock_assignments (s: list flat_stmnt): list flat_stmnt :=
-  snd (fold_left clock_assignment s (RTree.empty _, nil)).
+Fixpoint clock_stmnt (t: PTree.t expr) (f: stmnt): 
+    res (PTree.t expr * stmnt) :=
+  match f with
+  | Vblock (Vvar r) e => 
+    do fe <- clock_expr t e;
+    OK (PTree.set r fe t, (Vnonblock (Vvar r) fe))
+  | Vnonblock (Vvar r) e =>
+    (* let fe := clock_expr t e in  *)
+    (* OK (PTree.set r fe t, Vnonblock (Vvar r) fe) *)
+    Error (msg "ClockRegisters: no support for nonblocking assignment")
+  | Vseq a b => 
+    do (t', s') <- clock_stmnt t a;
+    do (t'', s'') <- clock_stmnt t' b;
+    OK (t'', Vseq s' s'')
+  | Vskip => OK (t, Vskip)
+  | Vblock (Vvari r e) e' => Error (msg "ClockRegisters: no support for arrays")
+  | Vnonblock (Vvari r e) e' => Error (msg "ClockRegisters: no support for nonblock arrays")
+  | Vblock _ e' => Error (msg "ClockRegisters: no support for other blocking assignment")
+  | Vnonblock _ e' => Error (msg "ClockRegisters: no support for other nonblocking assignment")
+  | Vcond _ _ _ => Error (msg "ClockRegisters: no support for cond")
+  | Vcase _ _ _ => Error (msg "ClockRegisters: no support for case")
+  end.
 
-Definition clock_stmnt_assignments (s: Verilog.stmnt): Errors.res Verilog.stmnt :=
-  do fs <- flatten_seq_block s;
-  ret (fold_seq_block (clock_assignments fs)).
+(* Definition clock_assignments (s: list stmnt): list stmnt := *)
+(*   snd (fold_left clock_assignment s (RTree.empty _, nil)). *)
+
+(* Definition clock_stmnt_assignments (s: Verilog.stmnt): Errors.res Verilog.stmnt := *)
+(*   do fs <- flatten_seq_block s; *)
+(*   ret (fold_seq_block (clock_assignments fs)). *)
+
+Lemma mfold_left_error:
+  forall A B f l m, @mfold_left A B f l (Error m) = Error m.
+Proof. now induction l. Qed.
+
+Lemma mfold_left_cons:
+  forall A B f a l x y, 
+    @mfold_left A B f (a :: l) x = OK y ->
+    exists x' y', @mfold_left A B f l (OK y') = OK y /\ f x' a = OK y' /\ x = OK x'.
+Proof.
+  intros.
+  destruct x; [|now rewrite mfold_left_error in H].
+  cbn in H.
+  replace (fold_left (fun (a : mon A) (b : B) => bind (fun a' : A => f a' b) a) l (f a0 a) = OK y) with
+    (mfold_left f l (f a0 a) = OK y) in H by auto.
+  destruct (f a0 a) eqn:?; [|now rewrite mfold_left_error in H].
+  eauto.
+Qed.
+
+Lemma mfold_left_app:
+  forall A B f a l x y, 
+    @mfold_left A B f (a ++ l) x = OK y ->
+    exists y', @mfold_left A B f a x = OK y' /\ @mfold_left A B f l (OK y') = OK y.
+Proof.
+  induction a.
+  - intros. destruct x; [|now rewrite mfold_left_error in H]. exists a. eauto.
+  - intros. destruct x; [|now rewrite mfold_left_error in H]. rewrite <- app_comm_cons in H.
+    exploit mfold_left_cons; eauto.
+Qed.
+
+Lemma transf_clock_stmnt_output :
+  forall l t t',
+    mfold_left (fun b a =>
+      do (_t, a') <- clock_stmnt (PTree.empty _) (snd a);
+      OK (PTree.set (fst a) a' b)) l (OK t) = OK t' ->
+    forall x,
+      ~ In x (List.map fst l) ->
+      t' ! x = t ! x.
+Proof.
+  induction l.
+  - cbn; intros. now inv H.
+  - intros.
+    exploit mfold_left_cons; eauto; simplify. inv H4. unfold bind2, bind in *.
+    repeat (destruct_match; try discriminate). inv H1.
+    assert (~ In x (List.map fst l)) by tauto.
+    assert (fst a <> x) by tauto.
+    assert ((PTree.set (fst a) s x0) ! x = x0 ! x) by (now rewrite PTree.gso by auto).
+    rewrite <- H4. eauto.
+Qed.
+
+Lemma transf_clock_stmnt_spec :
+  forall l t t',
+    mfold_left (fun b a =>
+      do (_t, a') <- clock_stmnt (PTree.empty _) (snd a);
+      OK (PTree.set (fst a) a' b)) l (OK t) = OK t' ->
+    list_norepet (List.map fst l) ->
+    forall x y,
+      In (x, y) l ->
+      exists tz z, clock_stmnt (PTree.empty _) y = OK (tz, z)
+                   /\ t' ! x = Some z.
+Proof.
+  induction l.
+  - intros. inv H1.
+  - intros. inv H1. exploit mfold_left_cons; eauto; simplify. inv H4. 
+    unfold bind, bind2 in *. repeat (destruct_match; try discriminate; []). inv H1.
+    do 2 eexists; split. eauto. inv H0. erewrite transf_clock_stmnt_output; eauto. 
+    now rewrite PTree.gss.
+    exploit mfold_left_cons; eauto; simplify. inv H5.
+    unfold bind, bind2 in *. repeat (destruct_match; try discriminate; []). inv H1.
+    inv H0. exploit IHl; eauto.
+Qed.
+
+Lemma transf_clock_stmnt_spec_in :
+  forall l t',
+    mfold_left (fun b a =>
+      do (_t, a') <- clock_stmnt (PTree.empty _) (snd a);
+      OK (PTree.set (fst a) a' b)) l (OK (PTree.empty _)) = OK t' ->
+    list_norepet (List.map fst l) ->
+    forall x y,
+      t' ! x = Some y ->
+      exists y', In (x, y') l.
+Proof.
+  intros. destruct (in_dec peq x (List.map fst l)).
+  - eapply in_map_iff in i; simplify. destruct x0; cbn in *. eauto.
+  - exploit transf_clock_stmnt_output; eauto; intros.
+    rewrite H1 in H2. rewrite PTree.gempty in H2. discriminate.
+Qed.
+
+Definition max_pc_map (m : Maps.PTree.t stmnt) :=
+  PTree.fold (fun m pc i => Pos.max m pc) m 1%positive.
+
+Lemma max_pc_map_sound:
+  forall m pc i, m!pc = Some i -> Ple pc (max_pc_map m).
+Proof.
+  intros until i. unfold max_pc_function.
+  apply PTree_Properties.fold_rec with (P := fun c m => c!pc = Some i -> Ple pc m).
+  (* extensionality *)
+  intros. apply H0. rewrite H; auto.
+  (* base case *)
+  rewrite PTree.gempty. congruence.
+  (* inductive case *)
+  intros. rewrite PTree.gsspec in H2. destruct (peq pc k).
+  inv H2. unfold Ple; lia.
+  apply Ple_trans with a. auto. unfold Ple; lia.
+Qed.
+
+Lemma max_pc_wf :
+  forall m, Z.pos (max_pc_map m) <= Integers.Int.max_unsigned ->
+            map_well_formed m.
+Proof.
+  unfold map_well_formed. intros.
+  exploit list_in_map_inv. eassumption. intros [x [A B]]. destruct x.
+  apply Maps.PTree.elements_complete in B. apply max_pc_map_sound in B.
+  unfold Ple in B. apply Pos2Z.pos_le_pos in B. subst.
+  simplify. transitivity (Z.pos (max_pc_map m)); eauto.
+Qed.
 
 Program Definition transf_module (m: DHTL.module) : Errors.res DHTL.module :=
-  do dp <- PTree.fold (fun b i a =>
-             do tb <- b;
-             do a' <- clock_stmnt_assignments a;
-             ret (PTree.set i a' tb)) m.(mod_datapath) (Errors.OK (PTree.empty _));
-  ret (mkmodule m.(mod_params)
-    dp
-    m.(mod_entrypoint)
-    m.(mod_st)
-    m.(mod_stk)
-    m.(mod_stk_len)
-    m.(mod_finish)
-    m.(mod_return)
-    m.(mod_start)
-    m.(mod_reset)
-    m.(mod_clk)
-    m.(mod_scldecls)
-    m.(mod_arrdecls)
-    m.(mod_ram) 
-    _
-    m.(mod_ordering_wf)
-    m.(mod_ram_wf)
-    m.(mod_params_wf)).
-Next Obligation.
-Admitted.
+  do dp <- mfold_left (fun b a =>
+             do (_t, a') <- clock_stmnt (PTree.empty _) (snd a);
+             OK (PTree.set (fst a) a' b)) (PTree.elements m.(mod_datapath)) (Errors.OK (PTree.empty _));
+  match zle (Z.pos (max_pc_map dp)) Integers.Int.max_unsigned with
+  | left LEDATA =>
+    OK (mkmodule m.(mod_params)
+      dp
+      m.(mod_entrypoint)
+      m.(mod_st)
+      m.(mod_stk)
+      m.(mod_stk_len)
+      m.(mod_finish)
+      m.(mod_return)
+      m.(mod_start)
+      m.(mod_reset)
+      m.(mod_clk)
+      m.(mod_scldecls)
+      m.(mod_arrdecls)
+      m.(mod_ram) 
+      (max_pc_wf _ LEDATA)
+      m.(mod_ordering_wf)
+      m.(mod_ram_wf)
+      m.(mod_params_wf))
+  | _ => Error (msg "ClockRegisters: Failed")
+  end.
 
 Definition transf_fundef := transf_partial_fundef transf_module.
 
